# Material: 
- [Аналитическая Геометрия и Линейная Алгебра](Analiticheskaya_geometria_i_lineynaya_algebra_2020_Umnov.pdf)
- [Slides](2024_AGLA1_Lecture_1.pdf)
# Geometric view (int $\mathbb{R}^{2} \  and \ \mathbb{R}^{3}$):
>[!abstract] Scalar / dot product: 
>$a*b = |a||b|\cos\theta$, where $\theta$ is the angle between $a$ and $b$.
  ![Photo|500](Pasted%20image%2020240903223757.png)
>[!Abstract] Scalar projection of vector $a$ on vector $b$  
>**A scalar:** $a_{b}=\|a\|\cos \theta$ 

>[!abstract] Orthogonal projection of vector $a$ on vector $b$ 
> **A vector:** $a_{b}= \hat{b}\|a\|\cos\theta$ 
  $\hat{b}$ is the *unit vector* in the direction on $b$
  >
  >**Explanation:**
  ![](Introduction.%20Vector%20Spaces.%20Linear%20Independence.%20Basis..md#^cdc541)
  > Orthogonal projection is a Scalar projection but we also add a direction to it using the unit vector of vector $\hat{b}$ 
# Algebraic view:
>[!abstract] Dot product
>Let $V$ be a vector space over $\mathbb{R}$.
>By a *dot product* on $V$ we mean a real valued function $u \cdot v$ on $V \times V \rightarrow \mathbb{R}$ which satisfies the following axioms:
>- $u\cdot v = v \cdot u,\ \forall u, v \in V$
>- $u\cdot (w + v) = u\cdot w + u\cdot v,\ \forall u,v,w\in V$
>- $(\lambda u) \cdot v = \lambda(u\cdot v),\ \forall u,v\in V, \lambda\in\mathbb{R}$
>- $u\cdot u \geq 0,\ \forall u \in V$
>- $u\cdot u = 0 \Leftrightarrow u=0$
>$$u\cdot v = a_{1}b_{1}+...+a_{n}b_{n}=\sum^{N}_{n=1}a_{n}b_{n}$$
>Where $u =\{a_{1},...,a_{n}\}$ and $v=\{b_{1},...,b_{n}\}$

> [!attention] Notation
> $u\cdot = (u,v) = u\ v = \langle u,v \rangle$
# Norm (or a length) of a vector:
> [!abstract] Definition
> We say $\| u \|$ is a norm on a vector space $V$ if $\forall u, v \in V$ and $\alpha\in\mathbb{R}:$
> - $\| \alpha u \| = |\alpha| \|u\|$
> - $\|u\| \geq 0$
> - $\| u \| = 0 \Leftrightarrow u = 0$
> - $\| u+v \| \leq\|u\| + \| v\|$

>[!Note] Equality
>$u\cdot v = \sum^{n}_{i=1}u_{i}v_{i} = \|u\|\|v\|\cos\theta$

>[!check] Proof
>![Drawing 2024-09-14 11.42.14.excalidraw](Drawing%202024-09-14%2011.42.14.excalidraw.md)
>$$\displaylines{\| V_{2}-V_{1}\|^{2}=\|V_{1}\|^{2}+\|V_{2}\|^{2}-2\|V_{1}\|\|V_{2}\| = \\(a_{1}^{2}+b_{1}^{2}+c_{1}^{2})+(a_{2}^{2}+b_{2}^{2}+c_{2}^{2})-2\|V_{1}\|\|V_{2}\cos\theta\\\texttt{On the other hand, } \\
>\| V_{2}-V_{1}\|^{2}=(a_{2}-a_{1})^{2}+(b_{2}-b_{1})^{2}+(c_{1}-c_{2})^{2}=\\
>a_{2}^{2}-2a_{2}a_{1}+a_{1}^{2}+b_{2}^{2}-2b_{2}b_{1}+b_{1}^{2}+c_{2}^{2}-2c_{2}c_{1}+c_{1}^{2}\\
>Thus, if we \\
>(a_{1}^{2}+b_{1}^{2}+c_{1}^{2})+(a_{2}^{2}+b_{2}^{2}+c_{2}^{2})-2\|V_{1}\|\|V_{2}\cos\theta=}$$
# Cauchy-Schwarz inequality:
> [!abstract] Cauchy-Schwarz inequality
> For all $x,y \in \mathbb{R^{n}},$$$|x\cdot y| \leq \|x\|\|y\|.$$

> [!check]- Proof
> Consider the expression $\| x- \lambda y \|^{2}.$ We must have $$\displaylines{\|x-\lambda y\|^{2}\geq 0\\
> (x-\lambda y)\cdot(x - \lambda y)\geq 0\\ 
> \lambda^{2}\|y\|^{2} - \lambda (2x \cdot y) + \|x\|^{2}\geq 0.}$$
> Viewing this as a quadratic in $\lambda$, we see that the quadratic is non-negative. It's possible if the discriminant $\Delta\leq0$, so quadratic cannot have 2 different real roots. $$\displaylines{\Delta = b^{2}-4ac\leq0 \\
> 4(x\cdot y)^{2}\leq 4\|y\|^{2}\|x\|^{2}\\
> (x\cdot y)^{2}\leq \|x\|^{2}\|y\|^{2}\\
> |x\cdot y|\leq\|x\|\|y\|}$$
# Triangle Inequality:
> [!abstract] Triangle inequality
> $\|x+y\|\leq\|x\|+\|y\|.$

>[!check]- Proof
>$$\|x+y\|^{2}= (x+y)\cdot(x+y)=\|x\|^{2}+2x\cdot y + \|y\|^{2}$$ $$\leq \|x\|^{2}+2\|x\|\|y\| + \|y\|^{2} = (\|x\|+\|y\|)^{2}$$ 

# Orthogonality
> [!abstract] Definition
> Let $V$ be vector space with a dot product.
> Vectors $u,v\in V$ are said to be **orthogonal** if $$u\cdot v =0$$
# Homework
- Show that the difference between a vector $a$ and its orthogonal projection ($a_{b}$) on a vector $b$ is orthogonal to the vector $b$.
  If $$p=a-a_{b}$$then $$p\cdot b=0$$
  **Solution:**
  $$p = a - a_{b} = a - \hat{b}\|a\|\cos\theta$$
  Substitute the $p$ in another equation: $$\displaylines{
  (a-\hat{b}\|a\|\cos\theta)\cdot b=0 \\
  a\cdot b - b\cdot \hat{b}\|a\|\cos\theta =0 \\
  \|a\|\|b\|\cos \theta - b\cdot \hat{b}\|a\| \cos\theta = 0
  }$$We know that $\hat{b} = \frac{b}{\|b\|} \Leftrightarrow b\cdot \hat{b}=\frac{b\cdot b}{\|b\|}=\frac{\|b\|^{2}}{\|b\|}= \|b\|$, if we substitude it into expression: $$\|a\|\|b\|\cos \theta-\|b\|\|a\|\cos\theta=0$$$\blacksquare$  
- In the triangle ABC the median AD is divided into three equal segments: AE, EF and FD. $$\displaylines{\overline{BA} \cdot \overline{CA}=4\\
   \overline{BF}\cdot\overline{CF}=-1}$$
   Find $\overline{BE}\cdot \overline{CE}$. 
   **Solution:**
	   ![Drawing 2024-09-09 23.41.39.excalidraw](Drawing%202024-09-09%2023.41.39.excalidraw.md)
$$\displaylines{\overline{AD} = \frac{1}{2}\cdot (\overline{AC}+\overline{AB})\\
\overline{AF} = \frac{2}{3}\overline{AD} = \frac{1}{3}(\overline{AC}+\overline{AB})}$$
$$\displaylines{
\overline{CA}+\overline{AF} = \overline{CF} = \overline{CA}+\frac{1}{3}(\overline{AB}+\overline{AC})=\frac{2}{3}\overline{CA}-\frac{1}{3}\overline{BA}\\
\overline{BF}=\overline{BA}+\frac{1}{3}(\overline{AB}+\overline{AC})=\frac{2}{3}\overline{BA}-\frac{1}{3}\overline{CA}}$$
$$\displaylines{
\overline{CE} = \frac{1}{2}(\overline{CA}+\overline{CF})=\frac{1}{2}(\overline{CA}+\frac{2}{3}\overline{CA}-\frac{1}{3}\overline{BA})
=\frac{5}{6}\overline{CA}-\frac{1}{6}\overline{BA}\\
\overline{BE} = \frac{5}{6}\overline{BA}-\frac{1}{6}\overline{CA}}$$
$$\displaylines{
\overline{CE}\cdot\overline{BE}=\frac{25}{36}\cdot 4 -\frac{5}{36}\overline{CA}^{2}- \frac{5}{36} \overline{BA}^{2}+ \frac{1}{36}\cdot 4 =\\ \frac{26}{9}- \frac{5}{36}(\overline{CA}^{2}+\overline{BA}^{2})
}$$
$$\displaylines{
\overline{BF}\cdot\overline{CF}= \frac{4}{9}\cdot 4 - \frac{2}{9}\overline{CA}^{2}- \frac{2}{9}\overline{BA}^{2}+ \frac{1}{9}\cdot 4 = \\
\frac{20}{9}- \frac{2}{9}(\overline{CA}^{2}+\overline{BA}^{2})=-1 \Rightarrow \\
\Rightarrow \overline{CA}^{2}+\overline{BA}^{2}= \frac{29}{2}
}$$
$$\displaylines{
\overline{CE}\cdot\overline{BE}= \frac{26}{9}- \frac{5}{36}\cdot \frac{29}{2} = \frac{26}{9}- \frac{145}{72} = \frac{26*8-145}{72}=\\
\frac{208-145}{72}=\frac{63}{72}=\frac{7}{8}
}$$ 